src/asn1/ASN1.Spec.BOOLEAN.fsti
@@ -27,7 +27,7 @@ val synth_asn1_boolean_inverse
   (requires True)
   (ensures fun b -> synth_asn1_boolean b == x)
 
-let parse_asn1_boolean_kind = strong_parser_kind 1 1 None
+let parse_asn1_boolean_kind = strong_parser_kind 1 1 (Some ParserKindMetadataTotal)
 val parse_asn1_boolean
 : parser parse_asn1_boolean_kind bool
 
@@ -53,3 +53,58 @@ val serialize_asn1_boolean_unfold
   `Seq.equal`
   serialize serialize_u8 (synth_asn1_boolean_inverse b))
 
+/// Specialized TLV
+///
+open ASN1.Spec.Tag
+open ASN1.Spec.Length
+
+val synth_asn1_boolean_TLV
+  (a: (the_asn1_type BOOLEAN * asn1_int32_of_tag BOOLEAN) * datatype_of_asn1_type BOOLEAN)
+: GTot (datatype_of_asn1_type BOOLEAN)
+
+val synth_asn1_boolean_TLV_inverse
+  (x: datatype_of_asn1_type BOOLEAN)
+: GTot (a: ((the_asn1_type BOOLEAN * asn1_int32_of_tag BOOLEAN) * datatype_of_asn1_type BOOLEAN){x == synth_asn1_boolean_TLV a})
+
+let parse_asn1_boolean_TLV_kind
+: parser_kind
+= parse_asn1_tag_kind
+  `and_then_kind`
+  parse_asn1_length_kind_of_tag BOOLEAN
+  `and_then_kind`
+  parse_asn1_boolean_kind
+
+val parse_asn1_boolean_TLV
+: parser parse_asn1_boolean_TLV_kind (datatype_of_asn1_type BOOLEAN)
+
+val parse_asn1_boolean_TLV_unfold
+  (input_TLV: bytes)
+: Lemma (
+  parse parse_asn1_boolean_TLV input_TLV ==
+ (match parse (parse_the_asn1_tag BOOLEAN) input_TLV with
+  | None -> None
+  | Some (BOOLEAN, consumed_T) ->
+    (let input_LV = Seq.slice input_TLV consumed_T (Seq.length input_TLV) in
+     match parse (parse_asn1_length_of_tag BOOLEAN) input_LV with
+     | None -> None
+     | Some (1ul, consumed_L) ->
+       (let input_V = Seq.slice input_LV consumed_L (Seq.length input_LV) in
+        match parse parse_asn1_boolean input_V with
+        | None -> None
+        | Some (value, consumed_V) -> Some (value, consumed_T + consumed_L + consumed_V))))
+)
+
+val serialize_asn1_boolean_TLV
+: serializer parse_asn1_boolean_TLV
+
+val serialize_asn1_boolean_TLV_unfold
+  (value: datatype_of_asn1_type BOOLEAN)
+: Lemma (
+  serialize serialize_asn1_boolean_TLV value
+  `Seq.equal`
+ (serialize (serialize_the_asn1_tag BOOLEAN) BOOLEAN
+  `Seq.append`
+  serialize (serialize_asn1_length_of_tag BOOLEAN) 1ul
+  `Seq.append`
+  serialize serialize_asn1_boolean value)
+)
